\documentclass{article}
\usepackage{geometry}        
\geometry{letterpaper}    
\usepackage[parfill]{parskip}  
\usepackage{hyperref}
\usepackage{graphicx}
\usepackage{amssymb}
\usepackage{epstopdf}
\usepackage{amsmath}
\pagestyle{empty}
 
\begin{document}
\baselineskip 2.7ex
\parskip 3.5ex


%Space/Indentation
\newcommand{\noi}{\noindent}
\newcommand{\vnu}{\vspace*{-1mm}}
\newcommand{\vnd}{\vspace*{-2mm}}
\newcommand{\vnt}{\vspace*{-3mm}}
\newcommand{\vnq}{\vspace*{-4mm}}
\newcommand{\vnc}{\vspace*{-5mm}}
\newcommand{\vu}{\vspace*{1mm}}
\newcommand{\vd}{\vspace*{2mm}}
\newcommand{\vt}{\vspace*{3mm}}
%\newcommand{\vq}{\vspace*{4mm}}
\newcommand{\vc}{\vspace*{5mm}}
\newcommand{\hs}{\hspace*{5mm}}

%Equations/Entries
\newcommand{\beq}{\begin{equation}}
\newcommand{\bequo}{\begin{quotation}}
\newcommand{\beqa}{\begin{eqnarray}}
\newcommand{\eeq}{\end{equation}}
\newcommand{\equo}{\end{quotation}}
\newcommand{\eeqa}{\end{eqnarray}}
\newcommand{\non}{\nonumber}
\newcommand{\mx}{\mbox}
\newcommand{\mxf}[1]{\mbox{\footnotesize{#1}}}
\newcommand{\lb}{\label}
\newcommand{\fr}[1]{(\ref{#1})}
\newtheorem{entry}{}[section]
\newcommand{\bent}[1]{\vspace*{-2cm}\hspace*{-1cm}\begin{entry}\lb{e{#1}}\rm}
\newcommand{\eent}{\end{entry}}
\newcommand{\fre}[1]{{\bf\ref{e{#1}}}}
\newcommand{\Emark}{$\sqcap\hspace{-2.7mm}\sqcup$}
\newcommand{\sEmark}{{\fns $\sqcap\hspace{-2.3mm}\sqcup$}}
\newcommand{\fn}{\footnote}


%Greek Letters
\renewcommand{\a}{\alpha}
\renewcommand{\b}{\beta}
\newcommand{\g}{\gamma}
\newcommand{\G}{\Gamma}
\renewcommand{\d}{\delta}
\renewcommand{\th}{\theta}
\newcommand{\Th}{\Theta}
\newcommand{\D}{\Delta}
\newcommand{\e}{\varepsilon}
\newcommand{\s}{\sigma}
\renewcommand{\S}{\Sigma}
\newcommand{\w}{\omega}
\newcommand{\W}{\Omega}
\newcommand{\al}{\alpha}
\newcommand{\bet}{\beta}
\newcommand{\gam}{\gamma}
\newcommand{\lam}{\lambda}
\newcommand{\Lam}{\Lambda}
\newcommand{\eps}{\varepsilon}
\newcommand{\ichi}\sichi
\renewcommand{\ni}{\sni}
\newcommand{\sichi}{{\mbox{{\footnotesize I}}}}
\newcommand{\sni}{{\mbox{{\footnotesize II}}}}

%Letter Style
%\renewcommand{\vec}{\bm}
\newcommand{\svec}[1]{\mbox{{\footnotesize $\bm{#1}$}}}
\newcommand{\bm}[1]{\mbox{\boldmath $#1$}}
\newcommand{\sbm}[1]{\small{\mbox{\boldmath $#1$}}}
\newcommand{\fns}{\footnotesize}
\newcommand{\ol}{\overline}
\newcommand{\ul}{\underline}
\newcommand{\vr}{\bm{r}}
\newcommand{\vq}{\bm{q}}
\newcommand{\vk}{\bm{k}}
\newcommand{\vx}{\bm{x}}
\newcommand{\vy}{\bm{y}}

%Arrows
\newcommand{\see}{$\rightarrow$}
\newcommand{\react}{$\longrightarrow$}
\newcommand{\map}{\rightarrow}
\newcommand{\pam}{\leftarrow}
\newcommand{\maps}{\rightarrow}
\newcommand{\imply}{\Rightarrow}
\newcommand{\Lrar}{\Leftrightarrow}
\newcommand{\rar}{\rightarrow}
\newcommand{\irrev}{\prec\prec}
\newcommand{\go}{\prec}
\newcommand{\adeq}{\stackrel{A}\sim}
\newcommand{\theq}{\stackrel{T}\sim}

%Derivatives
\newcommand{\pder}[2]{\frac{\partial {#1}}{\partial {#2}}}
\newcommand{\pdert}[2]{\frac{\partial^2 {#1}}{\partial {#2}^2}}
\newcommand{\fder}[2]{\frac{\delta {#1}}{\delta {#2}}}
\newcommand{\PDD}[3]{\left.\frac{\partial^{2}{#1}}{\partial{#2}^{2}}\right|_{#3}}
\newcommand{\PD}[3]{\left.\frac{\partial{#1}}{\partial{#2}}\right|_{#3}}
\newcommand{\der}[2]{\frac{d {#1}}{d {#2}}}

%Parentheses
\newcommand{\la}{\langle}
\newcommand{\ra}{\rangle}
\newcommand{\bra}[1]{\langle{#1}|}
\newcommand{\ket}[1]{|{#1}\rangle}
\newcommand{\FB}{${\bm \la\hspace{-.7mm}\la}$}  %footnote title start
\newcommand{\FE}{${\bm \ra\hspace{-.7mm}\ra}$}
\renewcommand{\v}{\vspace*{2mm}}
%logic
%\renewcommand{\or}{\vee} %this interferes with beqa/eeqa
\renewcommand{\and}{\wedge}

\renewcommand{\deg}{^\circ}
\newcommand{\com}{{\bf [C] }} 
\newcommand{\cend}{\Emark\[\]\vspace*{-1. cm}}
\newcommand{\x}{\times}

%tabbing
\newcommand{\MyTabs}{ \hspace*{25.mm} \= ... \kill }
%%%%%%%%

Note: $\mu$ is the observed expectation value, and $\sigma$ is the standard error of $\mu$.\\
For $\mu > 0$ condition:
\[
\begin{aligned}
	&P(x \ge 0|\mu_{opt}) = &&\frac{1}{\sigma\sqrt{2\pi}}e^{-\frac{(x-\mu_{opt})^2}{2\sigma^2}} = P(x \ge 0|\mu_{opt} = x) = \frac{1}{\sigma\sqrt{2\pi}}e^{-\frac{(x-x)^2}{2\sigma^2}}&& = \frac{1}{\sigma\sqrt{2\pi}}\\
	&P(x < 0|\mu_{opt}) = &&\frac{1}{\sigma\sqrt{2\pi}}e^{-\frac{(x-\mu_{opt})^2}{2\sigma^2}} = P(x < 0|\mu_{opt} = 0) = \frac{1}{\sigma\sqrt{2\pi}}e^{-\frac{(x-0)^2}{2\sigma^2}}&& = \frac{1}{\sigma\sqrt{2\pi}}e^{-\frac{x^2}{2\sigma^2}}\\
	&R(x \ge 0) =  &&P(x \ge 0|\mu)/P(x \ge 0|\mu_{opt}) =  \frac{1}{\sigma\sqrt{2\pi}}e^{-\frac{(x-\mu)^2}{2\sigma^2}}/\frac{1}{\sigma\sqrt{2\pi}}&& = e^{-\frac{(x-\mu)^2}{2\sigma^2}}\\
	&R(x < 0) =  &&P(x < 0|\mu)/P(x < 0|\mu_{opt}) =  \frac{1}{\sigma\sqrt{2\pi}}e^{-\frac{(x-\mu)^2}{2\sigma^2}}/\frac{1}{\sigma\sqrt{2\pi}}e^{-\frac{x^2}{2\sigma^2}}&& = e^{\frac{2x\mu - \mu^2}{2\sigma^2}}\\
\end{aligned}
\]
\[
	-x_u^2 + 2x_u\mu - \mu^2 = 2x_l\mu - \mu^2
\]
\[
	\Rightarrow -x_u^2 + 2x_u\mu  = 2x_l\mu
\]
\[
	\Rightarrow x_l = x_u - \frac{x_u^2}{2\mu}
\]

For $\mu < b$ condition:
\[
\begin{aligned}
	&P(x \le b|\mu_{opt}) = &&P(x \le b|\mu_{opt} = x) = \frac{1}{\sigma\sqrt{2\pi}}e^{-\frac{(x-x)^2}{2\sigma^2}}&& = \frac{1}{\sigma\sqrt{2\pi}}\\
	&P(x > b|\mu_{opt}) = &&P(x > b|\mu_{opt} = b)&& = \frac{1}{\sigma\sqrt{2\pi}}e^{-\frac{(x-b)^2}{2\sigma^2}}\\
	&R(x \le b) =  &&P(x \le b|\mu)/P(x \ge 0|\mu_{opt}) =  \frac{1}{\sigma\sqrt{2\pi}}e^{-\frac{(x-\mu)^2}{2\sigma^2}}/\frac{1}{\sigma\sqrt{2\pi}}&& = e^{-\frac{(x-\mu)^2}{2\sigma^2}}\\
	&R(x > b) =  &&P(x > b|\mu)/P(x < 0|\mu_{opt}) =  \frac{1}{\sigma\sqrt{2\pi}}e^{-\frac{(x-\mu)^2}{2\sigma^2}}/\frac{1}{\sigma\sqrt{2\pi}}e^{-\frac{(x-b)^2}{2\sigma^2}}&& = e^{\frac{(2x-(\mu+b))(\mu-b)}{2\sigma^2}}\\
\end{aligned}
\]
\[
	-x_u^2 + 2x_u\mu - \mu^2 = 2x_l(\mu-b) - \mu^2 + b^2
\]
\[
	\Rightarrow -x_u^2 + 2x_u\mu -b^2 = 2x_l(\mu-b)
\]
\[
	\Rightarrow x_l = \frac{2x_u\mu - x_u^2 - b^2}{2(\mu-b)}
\]

 \end{document} 




















